perf: use Array for CNF formulas (#11832)
This PR uses an `Array` instead of a `List` to store the clauses in
`Std.CNF`. This reduces the memory footprint and pressure on the
allocator, leading to noticeable performance changes with gigantic CNFs.

src/Std/Sat/AIG/CNF.lean
@@ -13,7 +13,6 @@ import Init.Omega
 
 public section
 
-
 /-!
 This module contains an implementation of a verified Tseitin transformation on AIGs. The key results
 are the `toCNF` function and the `toCNF_equisat` correctness statement. The implementation is
@@ -31,42 +30,43 @@ namespace Decl
 Produce a Tseitin style CNF for a `Decl.false`, using `output` as the tree node variable.
 -/
 def falseToCNF (output : α) : CNF α :=
-  [[(output, .false)]]
+  .empty |>.add [(output, .false)]
 
 /--
 Produce a Tseitin style CNF for a `Decl.atom`, using `output` as the tree node variable.
 -/
 def atomToCNF (output : α) (atom : α) : CNF α :=
-  [[(output, true), (atom, .false)], [(output, .false), (atom, true)]]
+  CNF.empty
+    |>.add [(output, true), (atom, .false)]
+    |>.add [(output, .false), (atom, true)]
 
 /--
 Produce a Tseitin style CNF for a `Decl.gate`, using `output` as the tree node variable.
 -/
 def gateToCNF (output : α) (lhs rhs : α) (linv rinv : Bool) : CNF α :=
-    -- a ↔ (b and c) as CNF: (¬a ∨ b) ∧ (¬a ∨ c) ∧ (a ∨ ¬b ∨ ¬c)
-    -- a ↔ (b and ¬c) as CNF: (¬a ∨ b) ∧ (¬a ∨ ¬c) ∧ (a ∨ ¬b ∨ c)
-    -- a ↔ (¬b and c) as CNF: (¬a ∨ ¬b) ∧ (¬a ∨ c) ∧ (a ∨ b ∨ ¬c)
-    -- a ↔ (¬b and ¬c) as CNF: (¬a ∨ ¬b) ∧ (¬a ∨ ¬c) ∧ (a ∨ b ∨ c)
-   [
-     [(output, .false), (lhs, !linv)],
-     [(output, .false), (rhs, !rinv)],
-     [(output, true),  (lhs, linv), (rhs, rinv)]
-   ]
+  -- a ↔ (b and c) as CNF: (¬a ∨ b) ∧ (¬a ∨ c) ∧ (a ∨ ¬b ∨ ¬c)
+  -- a ↔ (b and ¬c) as CNF: (¬a ∨ b) ∧ (¬a ∨ ¬c) ∧ (a ∨ ¬b ∨ c)
+  -- a ↔ (¬b and c) as CNF: (¬a ∨ ¬b) ∧ (¬a ∨ c) ∧ (a ∨ b ∨ ¬c)
+  -- a ↔ (¬b and ¬c) as CNF: (¬a ∨ ¬b) ∧ (¬a ∨ ¬c) ∧ (a ∨ b ∨ c)
+  CNF.empty
+    |>.add [(output, .false), (lhs, !linv)]
+    |>.add [(output, .false), (rhs, !rinv)]
+    |>.add [(output, true),  (lhs, linv), (rhs, rinv)]
 
 @[simp]
 theorem falseToCNF_eval :
     (falseToCNF output).eval assign
       =
     (assign output == .false) := by
-  simp [falseToCNF, CNF.eval, CNF.Clause.eval]
+  simp [falseToCNF]
 
 @[simp]
 theorem atomToCNF_eval :
     (atomToCNF output a).eval assign
       =
     (assign output == assign a) := by
-  simp only [atomToCNF, CNF.eval_cons, CNF.Clause.eval_cons, beq_true, beq_false,
-    CNF.Clause.eval_nil, Bool.or_false, CNF.eval_nil, Bool.and_true]
+  simp only [atomToCNF, CNF.eval_add, CNF.Clause.eval_cons, beq_false, beq_true,
+    CNF.Clause.eval_nil, Bool.or_false, CNF.eval_empty, Bool.and_true]
   cases assign output <;> cases assign a <;> decide
 
 @[simp]
@@ -74,8 +74,8 @@ theorem gateToCNF_eval :
     (gateToCNF output lhs rhs linv rinv).eval assign
       =
     (assign output == (((assign lhs) ^^ linv) && ((assign rhs) ^^ rinv))) := by
-  simp only [CNF.eval, gateToCNF, CNF.Clause.eval, List.all_cons, List.any_cons, beq_false,
-    List.any_nil, Bool.or_false, beq_true, List.all_nil, Bool.and_true]
+  simp only [gateToCNF, CNF.eval_add, CNF.Clause.eval_cons, beq_true, CNF.Clause.eval_nil,
+    Bool.or_false, beq_false, CNF.eval_empty, Bool.and_true]
   cases assign output
     <;> cases assign lhs
       <;> cases assign rhs
@@ -157,7 +157,7 @@ def Cache.Inv (cnf : CNF (CNFVar aig)) (marks : Array Bool)
 /--
 The `Cache` invariant always holds for an empty CNF when all nodes are unmarked.
 -/
-theorem Cache.Inv_init : Inv ([] : CNF (CNFVar aig)) (.replicate aig.decls.size false)
+theorem Cache.Inv_init : Inv (.empty : CNF (CNFVar aig)) (.replicate aig.decls.size false)
     (by simp) := by
   intro assign _ idx hbound hmark
   simp at hmark
@@ -245,7 +245,7 @@ theorem Cache.IsExtensionBy_set (cache1 : Cache aig cnf1) (cache2 : Cache aig cn
 /--
 A cache with no entries is valid for an empty CNF.
 -/
-def Cache.init (aig : AIG Nat) : Cache aig [] where
+def Cache.init (aig : AIG Nat) : Cache aig .empty where
   marks := .replicate aig.decls.size false
   hmarks := by simp
   inv := Inv_init
@@ -256,7 +256,7 @@ Add a `Decl.false` to a `Cache`.
 def Cache.addFalse (cache : Cache aig cnf) (idx : Nat) (h : idx < aig.decls.size)
     (htip : aig.decls[idx]'h = .false) :
     {
-      out : Cache aig (Decl.falseToCNF (.inr ⟨idx, h⟩) ++ cnf)
+      out : Cache aig (cnf ++ Decl.falseToCNF (.inr ⟨idx, h⟩))
         //
       Cache.IsExtensionBy cache out idx h
     } :=
@@ -275,7 +275,7 @@ def Cache.addFalse (cache : Cache aig cnf) (idx : Nat) (h : idx < aig.decls.size
           simp [denote_idx_false htip, projectRightAssign_property, heval]
         next heq =>
           simp only [CNF.eval_append, Decl.falseToCNF_eval, Bool.and_eq_true, beq_iff_eq] at heval
-          have := cache.inv assign heval.right idx hbound hmarked
+          have := cache.inv assign heval.left idx hbound hmarked
           rw [this]
     }
   ⟨out, IsExtensionBy_set cache out idx hmarkbound (by simp [out])⟩
@@ -286,7 +286,7 @@ Add a `Decl.atom` to a cache.
 def Cache.addAtom (cache : Cache aig cnf) (idx : Nat) (h : idx < aig.decls.size)
     (htip : aig.decls[idx]'h = .atom a) :
     {
-      out : Cache aig ((Decl.atomToCNF (.inr ⟨idx, h⟩) (.inl a)) ++ cnf)
+      out : Cache aig ((cnf ++ Decl.atomToCNF (.inr ⟨idx, h⟩) (.inl a)))
         //
       Cache.IsExtensionBy cache out idx h
     } :=
@@ -304,7 +304,7 @@ def Cache.addAtom (cache : Cache aig cnf) (idx : Nat) (h : idx < aig.decls.size)
           simp [heval, denote_idx_atom htip]
         next heq =>
           simp only [CNF.eval_append, Decl.atomToCNF_eval, Bool.and_eq_true, beq_iff_eq] at heval
-          have := cache.inv assign heval.right idx hbound hmarked
+          have := cache.inv assign heval.left idx hbound hmarked
           rw [this]
     }
   ⟨out, IsExtensionBy_set cache out idx hmarkbound (by simp [out])⟩
@@ -318,13 +318,14 @@ def Cache.addGate (cache : Cache aig cnf) {hlb} {hrb} (idx : Nat) (h : idx < aig
     {
       out : Cache
               aig
-              (Decl.gateToCNF
+              (cnf ++
+                Decl.gateToCNF
                 (.inr ⟨idx, h⟩)
                 (.inr ⟨lhs.gate, by have := aig.hdag h htip; omega⟩)
                 (.inr ⟨rhs.gate, by have := aig.hdag h htip; omega⟩)
                 lhs.invert
                 rhs.invert
-                ++ cnf)
+                )
         //
       Cache.IsExtensionBy cache out idx h
     } :=
@@ -341,15 +342,15 @@ def Cache.addGate (cache : Cache aig cnf) {hlb} {hrb} (idx : Nat) (h : idx < aig
         next heq =>
           simp only [heq, CNF.eval_append, Decl.gateToCNF_eval, Bool.and_eq_true, beq_iff_eq]
             at htip heval
-          have hleval := cache.inv assign heval.right lhs.gate (by omega) hl
-          have hreval := cache.inv assign heval.right rhs.gate (by omega) hr
+          have hleval := cache.inv assign heval.left lhs.gate (by omega) hl
+          have hreval := cache.inv assign heval.left rhs.gate (by omega) hr
           simp only [denote_idx_gate htip, Bool.bne_false, projectRightAssign_property, heval]
           generalize lhs.invert = linv
           generalize rhs.invert = rinv
           cases linv <;> cases rinv <;> simp [hleval, hreval]
         next heq =>
           simp only [CNF.eval_append, Decl.gateToCNF_eval, Bool.and_eq_true, beq_iff_eq] at heval
-          have := cache.inv assign heval.right idx hbound hmarked
+          have := cache.inv assign heval.left idx hbound hmarked
           rw [this]
     }
   ⟨out, IsExtensionBy_set cache out idx hmarkbound (by simp [out])⟩
@@ -364,7 +365,7 @@ def State.Inv (cnf : CNF (CNFVar aig)) : Prop :=
 /--
 The `State` invariant always holds when we have an empty CNF.
 -/
-theorem State.Inv_nil : State.Inv ([] : CNF (CNFVar aig)) := by
+theorem State.Inv_nil : State.Inv (.empty : CNF (CNFVar aig)) := by
   simp [State.Inv]
 
 /--
@@ -434,7 +435,7 @@ structure State (aig : AIG Nat) where
 An initial state with no CNF clauses and an empty cache.
 -/
 def State.empty (aig : AIG Nat) : State aig where
-  cnf := []
+  cnf := .emptyWithCapacity (aig.decls.size * 2)
   cache := Cache.init aig
   inv := State.Inv_nil
 
@@ -477,7 +478,7 @@ def State.addFalse (state : State aig) (idx : Nat) (h : idx < aig.decls.size)
   let newCnf := Decl.falseToCNF (.inr ⟨idx, h⟩)
   have hinv := toCNF.State.Inv_falseToCNF htip
   let ⟨cache, hcache⟩ := cache.addFalse idx h htip
-  ⟨⟨newCnf ++ cnf, cache, State.Inv_append hinv inv⟩, by simp [newCnf, hcache]⟩
+  ⟨⟨cnf ++ newCnf, cache, State.Inv_append inv hinv⟩, by simp [newCnf, hcache]⟩
 
 /--
 Add the CNF for a `Decl.atom` to the state.
@@ -489,7 +490,7 @@ def State.addAtom (state : State aig) (idx : Nat) (h : idx < aig.decls.size)
   let newCnf := Decl.atomToCNF (.inr ⟨idx, h⟩) (.inl a)
   have hinv := toCNF.State.Inv_atomToCNF htip
   let ⟨cache, hcache⟩ := cache.addAtom idx h htip
-  ⟨⟨newCnf ++ cnf, cache, State.Inv_append hinv inv⟩, by simp [newCnf, hcache]⟩
+  ⟨⟨cnf ++ newCnf, cache, State.Inv_append inv hinv⟩, by simp [newCnf, hcache]⟩
 
 /--
 Add the CNF for a `Decl.gate` to the state.
@@ -509,7 +510,7 @@ def State.addGate (state : State aig) {hlb} {hrb} (idx : Nat) (h : idx < aig.dec
       rhs.invert
   have hinv := toCNF.State.Inv_gateToCNF htip
   let ⟨cache, hcache⟩ := cache.addGate idx h htip hl hr
-  ⟨⟨newCnf ++ cnf, cache, State.Inv_append hinv inv⟩, by simp [newCnf, hcache]⟩
+  ⟨⟨cnf ++ newCnf, cache, State.Inv_append inv hinv⟩, by simp [newCnf, hcache]⟩
 
 /--
 Evaluate the CNF contained within the state.
@@ -556,7 +557,7 @@ Convert an AIG into CNF, starting at some entry node.
 -/
 def toCNF (entry : Entrypoint Nat) : CNF Nat :=
   let ⟨state, _⟩ := go entry.aig entry.ref.gate entry.ref.hgate (toCNF.State.empty entry.aig)
-  let cnf : CNF (CNFVar entry.aig) := [(.inr ⟨entry.ref.gate, entry.ref.hgate⟩, !entry.ref.invert)] :: state.cnf
+  let cnf : CNF (CNFVar entry.aig) := state.cnf.add [(.inr ⟨entry.ref.gate, entry.ref.hgate⟩, !entry.ref.invert)]
   cnf.relabel inj
 where
   inj {aig : AIG Nat} (var : CNFVar aig) : Nat :=
@@ -661,7 +662,7 @@ Connect SAT results about the AIG to SAT results about the CNF.
 private theorem toCNF.denote_as_go {assign : AIG.CNFVar aig → Bool} :
     (⟦aig, ⟨start, inv, h1⟩, projectLeftAssign assign⟧ = false)
       →
-    CNF.eval assign (([(.inr ⟨start, h1⟩, !inv)] :: (go aig start h1 (.empty aig)).val.cnf)) = false := by
+    CNF.eval assign (((go aig start h1 (.empty aig)).val.cnf.add [(.inr ⟨start, h1⟩, !inv)])) = false := by
   intro h
   match heval1:(go aig start h1 (State.empty aig)).val.cnf.eval assign with
   | true =>
